src/Computation/ApplyMonad.v
@@ -1,17 +1,18 @@
 (** * A variant of the [Comp] monad laws using [apply] *)
 Require Import Coq.Strings.String Coq.Sets.Ensembles.
 Require Import Fiat.Common.
-Require Import Fiat.Computation.Core Fiat.Computation.Monad Fiat.Computation.SetoidMorphisms.
+Require Import Fiat.Computation.Core Fiat.Computation.Monad .
+(* Require Import Fiat.Computation.Core Fiat.Computation.Monad Fiat.Computation.SetoidMorphisms. *)
 
 (** ** Helper monad laws, on the left side of a [refine] *)
 
 Section monad.
-  Local Ltac t := let H := fresh in intro H; autorewrite with refine_monad; exact H.
+  Local Ltac t := unfold refineEq; let H := fresh in intro H; autorewrite with refine_monad; exact H.
 
   Lemma refine_bind_bind_helper X Y Z (f : X -> Comp Y) (g : Y -> Comp Z) x y
-  : refine (Bind x (fun u => Bind (f u) g)) y
-    -> refine (Bind (Bind x f) g) y.
-  Proof. t. Qed.
+  : refineEq (Bind x (fun u => Bind (f u) g)) y
+    -> refineEq (Bind (Bind x f) g) y.
+  Proof. unfold refineEq. let H := fresh in intro H.  t. Qed.
 
   Lemma refine_bind_unit_helper X Y (f : X -> Comp Y) x y
   : refine (f x) y
@@ -91,12 +92,12 @@ Ltac interleave_autorewrite_refine_monad_with tac :=
   repeat first [ reflexivity
                | progress tac
                | progress autorewrite with refine_monad
-               (*| rewrite refine_bind_bind'; progress tac
-               | rewrite refine_bind_unit'; progress tac
-               | rewrite refine_unit_bind'; progress tac
-               | rewrite <- refine_bind_bind; progress tac
-               | rewrite <- refine_bind_unit; progress tac
-               | rewrite <- refine_unit_bind; progress tac ]*)
+               (*| rewrite refine_bind_bind'; progress tac *)
+(*                | rewrite refine_bind_unit'; progress tac *)
+(*                | rewrite refine_unit_bind'; progress tac *)
+(*                | rewrite <- refine_bind_bind; progress tac *)
+(*                | rewrite <- refine_bind_unit; progress tac *)
+(*                | rewrite <- refine_unit_bind; progress tac ]*)
                | rewrite <- !refineEquiv_bind_bind; progress tac
                | rewrite <- !refineEquiv_bind_unit; progress tac
                | rewrite <- !refineEquiv_unit_bind; progress tac
