Makefile
@@ -163,13 +163,13 @@ ML4_OR_MLG := mlg
 EXTRA_PIPE_SED_FOR_COQPROJECT += | sed 's/@META@/META.coq-fiat-parsers/g'
 else
 # >= 8.5 if it exists
-NOT_EXISTS_LOC_DUMMY_LOC := $(call test_exists_ml_function,Loc.dummy_loc)
+# NOT_EXISTS_LOC_DUMMY_LOC := $(call test_exists_ml_function,Loc.dummy_loc)
 
-ifeq ($(NOT_EXISTS_LOC_DUMMY_LOC),1) # <= 8.4
-EXPECTED_EXT:=.v84
-ML_DESCRIPTION := "Coq v8.4"
-ML4_OR_MLG := ml4
-else
+# ifeq ($(NOT_EXISTS_LOC_DUMMY_LOC),1) # <= 8.4
+# EXPECTED_EXT:=.v84
+# ML_DESCRIPTION := "Coq v8.4"
+# ML4_OR_MLG := ml4
+# else
 ifdef COQ_VERSION # if not, we're just going to remake the relevant Makefile to include anyway, so we shouldn't error
 $(warning Unrecognized Coq version $(COQ_VERSION))
 EXPECTED_EXT:=.v819
@@ -178,7 +178,7 @@ OTHERFLAGS += -w "-deprecated-appcontext -notation-overridden"
 ML4_OR_MLG := mlg
 EXTRA_PIPE_SED_FOR_COQPROJECT += | sed 's/@META@/META.coq-fiat-parsers/g'
 
-endif
+# endif
 endif
 endif
 endif
